ListAdd.v
@@ -1,0 +1,49 @@
+Require Import List.
+Require Import RelationClasses.
+
+Section incl.
+  
+  Lemma incl_app_iff {A:Type} (l m n : list A) :
+    incl (l ++ m) n <-> incl l n /\ incl m n.
+  Proof.
+    unfold incl; intuition.
+    rewrite in_app_iff in H.
+    intuition.
+  Qed.
+  
+  Global Instance incl_pre A : PreOrder (@incl A).
+  Proof.
+    unfold incl.
+    constructor; red; intuition.
+  Qed.
+  Print incl.
+
+  Lemma incl_dec {A} (dec:forall a b:A, {a = b} + {a <> b}) (l1 l2:list A) :
+    {incl l1 l2} + {~ incl l1 l2}.
+  Proof.
+    unfold incl.
+    induction l1.
+    - left; inversion 1.
+    - destruct IHl1.
+      + destruct (in_dec dec a l2).
+        * left; simpl; intros; intuition; congruence.
+        * right; simpl;  intros inn; apply n; intuition.
+      + right; simpl; intros inn; apply n; intuition.
+  Defined.
+
+  Lemma nincl_exists {A} (dec:forall a b:A, {a = b} + {a <> b}) (l1 l2:list A) :
+      ~ incl l1 l2 -> {x | In x l1 /\ ~ In x l2}.
+    Proof.
+      unfold incl.
+      induction l1; simpl.
+      - intros H; elim H;  intuition.
+      - intros.
+        destruct (in_dec dec a l2).
+        + destruct IHl1.
+          * intros inn.
+            apply H. intuition; subst; trivial.
+          * exists x; intuition.
+        + exists a; intuition.
+    Qed.
+
+End incl.
